LocusType.v
@@ -59,127 +59,6 @@ Fixpoint find_pos' (p:posi) (l:list (var*nat*nat)) (pos:nat) :=
    end.
 Definition find_pos p l := find_pos' p l 0.
 
-(*
-Definition look_tenv (env:tenv) (x:posi) := (snd env) (find_pos x (fst env)).
-Definition look_range (env:tenv) (x:var) :=
-      match find_range x (fst env) with None => None
-              | Some pos => Some (lshift_fun (cut_n (snd env) (snd pos)) (fst pos))
-      end.
-Definition up_range (env:tenv) (x:var) (f:rz_val) :=
-    match find_range x (fst env) with None => env
-             | Some pos =>
-         (fst env, fun i => if i <? (fst pos) then (snd env) i 
-                            else if ((fst pos) <=? i) && (i <? snd pos)
-                            then f i else (snd env) i)
-    end.
-
-Definition flip_i (l:rz_val) (i:nat) := update l i (negb (l i)).
-Definition exchange (env:tenv) (p:posi) :=
-    let pos := (find_pos p (fst env)) in (fst env, flip_i (snd env) pos).
-
-Definition up_phase_phi (tenv:tenv) (x:var) (n:nat) :=
-  match look_range tenv x with None => None
-          | Some f => Some (up_range tenv x (rotate f n)) end.
-
-Definition up_phase_phi_r (tenv:tenv) (x:var) (n:nat) :=
-  match look_range tenv x with None => None
-          | Some f => Some (up_range tenv x (r_rotate f n)) end.
-*)
-(*
-Definition up_phase (tenv:tenv) (x:var) (q:nat) :=
-  match tenv x with (r,l) => update tenv x (rotate r q,l) end.
-
-Definition up_phase_r (tenv:tenv) (x:var) (q:nat) :=
-  match tenv x with (r,l) => update tenv x (r_rotate r q,l) end.
-
-Definition up_phase_phi (tenv:tenv) (x:var) (n:nat) :=
-  match tenv x with (r,q) => update tenv x (r, (rotate q n)) end.
-
-Definition up_phase_phi_r (tenv:tenv) (x:var) (n:nat) :=
-  match tenv x with (r, q) => update tenv x (r, (r_rotate q n)) end.
-
-Fixpoint list_in (l:list var) (x:var) := match l with [] => false | (y::yl) => if x =? y then true else list_in yl x end.
-
-Definition list_subset (al bl :list var) := (forall x, In x al -> In x bl).
-*)
-
-(*
-Fixpoint oqasm_type (qenv: var -> nat) (tv:tenv) (e:exp) :=
-   match e with SKIP x a => Some tv
-              | (X x (Num v)) => Some (exchange tv (x,v))
-              | (CU x (Num v) e) => if look_tenv tv (x,v) then oqasm_type qenv tv e else Some tv
-              | (RZ q x (Num v)) => Some tv
-              | (RRZ q x (Num v)) => Some tv
-              | (SR n x) => (up_phase_phi tv x (S n))
-              | (SRR n x) => (up_phase_phi_r tv x (S n))
-              | (QFT x b) => Some tv
-              | RQFT x b => Some tv
-              | Seq s1 s2 => match oqasm_type qenv tv s1 with Some tv1 => oqasm_type qenv tv1 s2 | _ => None end
-              | _ => Some tv
-   end.
-
-Definition gen_ch_set (qenv: var -> nat) (st:nat -> rz_val) (s:locus) (e:exp) :=
-    fun i => match oqasm_type qenv (s, (st i)) e
-             with Some tv => snd tv
-                | None => allfalse
-             end.
-
-Definition double_type (m:nat) (t t': type_cfac) :=
-   fun i => if i <? m then (fb_push false (t i)) else fb_push true (t' (i-m)).
-
-Definition get_core_ses (b:bexp) :=
-    match b with BEq c d x (Num v) => Some (x,v,v+1)
-               | BLt c d x (Num v) => Some (x,v,v+1)
-               | _ => None
-    end.
-
-Definition eval_bexp_set (b:bexp) (y:var) (v:nat) :=
-    match b with BEq (AExp (BA x)) (AExp (Num a)) i t => if x =? y then Some (v =? a) else None
-               | BLt (AExp (BA x)) (AExp (Num a)) i t => if x =? y then Some (v <? a) else None
-               | _ => None
-    end.
-
-Definition form_bits (n:nat) (t t':rz_val) (a:bool) := 
-               fun i => if i <? n then t i else fb_push a t' (i-n).
-
-Definition flat_type (x:var) (n:nat) (b:bexp) (a:bool) (t t': type_cfac) :=
-   fun i => match eval_bexp_set b x (a_nat2fb (t i) n)
-        with None => allfalse
-           | Some true => if a then form_bits n (t i) (lshift_fun (t' i) n) a
-                               else form_bits n (t i) (lshift_fun (t i) n) (negb a)
-           | Some false => if a then form_bits n (t i) (lshift_fun (t i) n) (negb a)
-                                else form_bits n (t i) (lshift_fun (t' i) n) a
-        end.
-
-Definition gen_diff_set (n:nat) (size:nat) (c:rz_val) :=
-   fun i => if i <? n then (fun j => if j <? size then (nat2fb i) j else c j) else allfalse.
-
-Fixpoint add_elem_set' (m size n:nat) (acc:type_cfac) (c:rz_val) :=
-    match m with 0 => (size+1,update acc size c)
-              | S i => if a_nat2fb (acc i) n =? a_nat2fb c n then (size,acc) else add_elem_set' i size n acc c
-    end.
-Definition add_elem_set (n:nat) (acc:nat*type_cfac) (c:rz_val) := add_elem_set' (fst acc) (fst acc) n (snd acc) c.
-
-Fixpoint add_n_elems (n:nat) (size:nat) (acc:nat * type_cfac) (addt:type_cfac) :=
-   match n with 0 => acc
-             | S i => add_n_elems i size (add_elem_set size acc (addt i)) addt
-   end.
-
-Fixpoint cal_set' (m:nat) (n:nat) (size:nat) (c:type_cfac) (acc:nat * type_cfac) :=
-   match m with 0 => acc
-            | S i => cal_set' i n size c (add_n_elems (2^n) size acc (gen_diff_set (2^n) n (c i)))
-   end.
-Definition cal_set (m n size:nat) (c:type_cfac) := cal_set' m n size c (0,fun i => allfalse).
-
-Inductive add_to_types' : type_map -> type_map -> type_map -> Prop :=
-   add_to_empty: forall T, add_to_types' T [] T
- | add_to_many_1: forall T T' s t T1, In s (dom T) -> add_to_types' T T' T1 -> add_to_types' T ((s,t)::T') T1
- | add_to_many_2: forall T T' s t T1, ~ In s (dom T) -> add_to_types' T T' T1 -> add_to_types' T ((s,t)::T') ((s,t)::T1).
-
-Inductive add_to_types : type_map -> type_map -> type_map -> Prop :=
-   add_to_type_rule: forall T T1 T2 T3, env_equiv T1 T2 -> add_to_types' T T2 T3 -> add_to_types T T1 T3.
-*)
-
 Inductive add_to_types' : type_map -> type_map -> type_map -> Prop :=
    add_to_empty: forall T, add_to_types' T [] T
  | add_to_many_1: forall T T' s t T1, In s (dom T) -> add_to_types' T T' T1 -> add_to_types' T ((s,t)::T') T1
@@ -202,6 +81,7 @@ Inductive perm_envs: type_map -> type_map -> Prop :=
    perm_env_empty: forall T, perm_envs T T
  | perm_env_many: forall T1 T2 T3, perm_env T1 T2 -> perm_envs T2 T3 -> perm_envs T1 T3.
 
+Axiom perm_envs_sym: forall T1 T2, perm_envs T1 T2 -> perm_envs T2 T1.
 
 Lemma perm_env_is_equiv: forall T1 T2, perm_envs T1 T2 -> env_equiv T1 T2.
 Proof.
@@ -301,7 +181,7 @@ Inductive locus_system {rmax:nat}
            : mode -> aenv -> type_map -> pexp -> type_map -> Prop :=
 
     | eq_ses : forall q env s T T' T1,
-         locus_system q env T s T' -> perm_envs T' T1 -> locus_system q env T s T1
+         locus_system q env T s T' -> env_equiv T' T1 -> locus_system q env T s T1
 
     | sub_ses: forall q env s T T' T1,
         locus_system q env T s T' -> locus_system q env (T++T1) s (T'++T1)
@@ -323,29 +203,13 @@ Inductive locus_system {rmax:nat}
                     locus_system q env ([([a], TNor)]) (AppSU (RH p)) ([([a], THad)])
     | appu_ses_h_had:  forall q env p a m, type_vari env p (QT m, [a]) -> simp_varia env p a ->
                     locus_system q env ([([a], THad)]) (AppSU (RH p)) ([([a], TNor)])
-(*
-    | appu_ses_h_ch:  forall q env T p l l' m, type_vari env p (QT m, l)
-                  -> find_type T l (Some (l',(CH))) ->
-                    locus_system q env T (AppSU (RH p)) ([(l', ((CH)))])
-    | appu_ses_qft_nor:  forall q env T x l m, AEnv.MapsTo x (QT m) env ->
-                  find_type T l (Some (l,(TNor))) ->
-                    locus_system q env T (AppSU (SQFT x)) ([(l, ((THad)))])
-    | appu_ses_qft_ch:  forall q env T x l l' t m, AEnv.MapsTo x (QT m) env ->
-                  find_type T l (Some (l',t)) ->
-                    locus_system q env T (AppSU (SQFT x)) ([(l', (CH))])
-    | appu_ses_rqft_nor:  forall q env T x l m, AEnv.MapsTo x (QT m) env ->
-                  find_type T l (Some (l,(TNor))) ->
-                    locus_system q env T (AppSU (SRQFT x)) ([(l, ((THad)))])
-    | appu_ses_rqft_ch:  forall q env T x l l' t m, AEnv.MapsTo x (QT m) env ->
-                  find_type T l (Some (l',t)) ->
-                    locus_system q env T (AppSU (SRQFT x)) ([(l', (CH))])
-*)
+
+    | appu_ses_h_ch:  forall q env p a l m, type_vari env p (QT m, [a]) -> simp_varia env p a ->
+                    locus_system q env ([([a]++l, CH)]) (AppSU (RH p)) ([([a]++l, CH)])
+
     | qif_ses: forall q env T b e, type_bexp env b (CT,nil) ->
                       locus_system q env T e T -> locus_system q env T (If b e) T
-(*
-    | qif_ses_m: forall env T b e T', type_bexp env b (Mo MT,nil) -> 
-                locus_system CT env T e T' -> locus_system CT env T (If b e) T'
-*)
+
     | qif_ses_ch: forall q env b n l l1 e, type_bexp env b (QT n,l) ->
                 locus_system QM env ([(l1,CH)]) e ([(l1,CH)])
              -> locus_system q env ([(l++l1,CH)]) (If b e) ([(l++l1,CH)])
